Changed the CompCert assembly to use instructions with its size information attached and changed the PC contain the actual PC

x86/Asm.v
@@ -291,7 +291,8 @@ Inductive instruction: Type :=
   | Psubl_ri (rd: ireg) (n: int)
   | Psubq_ri (rd: ireg) (n: int64).
 
-Definition code := list instruction.
+Definition instr_with_info:Type := instruction * ptrofs. (* Instruction with its size *)
+Definition code := list instr_with_info.
 Record function : Type := mkfunction { fn_sig: signature; fn_code: code; fn_frame: frame_info }.
 Definition fundef := AST.fundef function.
 Definition program := AST.program fundef unit.
@@ -362,6 +363,7 @@ Section RELSEM.
 
 
 Class FindLabels {function instructionx}
+  (instr_size : instructionx -> Z)
   (is_label : label -> instructionx -> bool)
   (fn_code : function -> list instructionx).
 
@@ -370,38 +372,46 @@ Class FindLabels {function instructionx}
 Fixpoint find_instr `{Hfl: FindLabels} (pos: Z) (c: list instructionx) {struct c} : option instructionx :=
   match c with
   | nil => None
-  | i :: il => if zeq pos 0 then Some i else find_instr (pos - 1) il
+  | i :: il => if zeq pos 0 then Some i else find_instr (pos - instr_size i) il
   end.
 
 (** Position corresponding to a label *)
 
-Definition is_label (lbl: label) (instr: instruction) : bool :=
+Definition is_label (lbl: label) (instr: instr_with_info) : bool :=
+  let instr := fst (instr) in
   match instr with
   | Plabel lbl' => if peq lbl lbl' then true else false
   | _ => false
   end.
 
-Global Instance: FindLabels is_label fn_code.
+Definition instr_size (i: instr_with_info) : Z :=
+  Ptrofs.unsigned (snd i).
 
-Lemma is_label_correct:
-  forall lbl instr,
-  if is_label lbl instr then instr = Plabel lbl else instr <> Plabel lbl.
-Proof.
-  intros.  destruct instr; simpl; try discriminate.
-  case (peq lbl l); intro; congruence.
-Qed.
+Global Instance: FindLabels instr_size is_label fn_code.
+
+(* Lemma is_label_correct: *)
+(*   forall lbl instr, *)
+(*   if is_label lbl instr then instr = Plabel lbl else instr <> Plabel lbl. *)
+(* Proof. *)
+(*   intros.  destruct instr; simpl; try discriminate. *)
+(*   case (peq lbl l); intro; congruence. *)
+(* Qed. *)
 
 
 Section WITH_FIND_LABELS.
-  Context {function instructionx is_label fn_code}
-          `{Hfl: FindLabels function instructionx is_label fn_code}.
+  Context {function instructionx instr_size is_label fn_code}
+          `{Hfl: FindLabels function instructionx instr_size is_label fn_code}.
 
-  Fixpoint label_pos `{Hfl: FindLabels function instructionx is_label fn_code} (lbl: label) (pos: Z) (c: list instructionx) {struct c} : option Z :=
+  Fixpoint label_pos `{Hfl: FindLabels function instructionx instr_size is_label fn_code}
+     (lbl: label) (pos: Z) (c: list instructionx) {struct c} : option Z :=
   match c with
   | nil => None
   | instr :: c' =>
-      if is_label lbl instr then Some (pos + 1) else label_pos lbl (pos + 1) c'
+    let nextpos := pos + instr_size instr in
+      if is_label lbl instr then Some nextpos else label_pos lbl nextpos c'
   end.
+
+End WITH_FIND_LABELS.
 
   Section WITHGE.
     Context {F V : Type}.
@@ -586,11 +596,17 @@ Inductive outcome {memory_model_ops: Mem.MemoryModelOps mem}: Type :=
   [nextinstr_nf] is a variant of [nextinstr] that sets condition flags
   to [Vundef] in addition to incrementing the [PC]. *)
 
-Definition nextinstr (rs: regset) :=
-  rs#PC <- (Val.offset_ptr rs#PC Ptrofs.one).
+(** The manipulation of PC is parameterized by a mapping from 
+    instructions to their actual sizes when compiled to machine-level bytes.
+    It is used to calculated the changes of PC as in the machine code.
+    It will be instantiated by the later phases of the transformation. *)
 
-Definition nextinstr_nf (rs: regset) : regset :=
-  nextinstr (undef_regs (CR ZF :: CR CF :: CR PF :: CR SF :: CR OF :: nil) rs).
+
+Definition nextinstr (rs: regset) (sz: ptrofs):=
+  rs#PC <- (Val.offset_ptr rs#PC sz).
+
+Definition nextinstr_nf (rs: regset) (sz: ptrofs) : regset :=
+  nextinstr (undef_regs (CR ZF :: CR CF :: CR PF :: CR SF :: CR OF :: nil) rs) sz.
 
 Definition goto_label {F V} (ge: Genv.t F V) (f: function) (lbl: label) (rs: regset) (m: mem) :=
   match label_pos lbl 0 (fn_code f) with
@@ -613,8 +629,8 @@ mode. *)
 
 Class MemAccessors
       `{!Mem.MemoryModelOps mem}
-      (exec_load: forall F V: Type, Genv.t F V -> memory_chunk -> mem -> addrmode -> regset -> preg -> outcome)
-      (exec_store: forall F V: Type, Genv.t F V -> memory_chunk -> mem -> addrmode -> regset -> preg -> list preg -> outcome)
+      (exec_load: forall F V: Type, Genv.t F V -> memory_chunk -> mem -> addrmode -> regset -> preg -> ptrofs -> outcome)
+      (exec_store: forall F V: Type, Genv.t F V -> memory_chunk -> mem -> addrmode -> regset -> preg -> list preg -> ptrofs -> outcome)
 : Prop := {}.
 
 Section MEM_ACCESSORS_DEFAULT.
@@ -624,18 +640,18 @@ care about kernel vs. user mode, and uses its memory model to define
 its memory accessors. *)
 
 Definition exec_load {F V} (ge: Genv.t F V) (chunk: memory_chunk) (m: mem)
-                     (a: addrmode) (rs: regset) (rd: preg) :=
+                     (a: addrmode) (rs: regset) (rd: preg) (sz:ptrofs):=
   match Mem.loadv chunk m (eval_addrmode ge a rs) with
-  | Some v => Next (nextinstr_nf (rs#rd <- v)) m
+  | Some v => Next (nextinstr_nf (rs#rd <- v) sz) m 
   | None => Stuck
   end.
 
 Definition exec_store {F V} (ge: Genv.t F V) (chunk: memory_chunk) (m: mem)
                       (a: addrmode) (rs: regset) (r1: preg)
-                      (destroyed: list preg) :=
+                      (destroyed: list preg) (sz:ptrofs) :=
   match Mem.storev chunk m (eval_addrmode ge a rs) (rs r1) with
   | Some m' =>
-    Next (nextinstr_nf (undef_regs destroyed rs)) m'
+    Next (nextinstr_nf (undef_regs destroyed rs) sz) m'
   | None => Stuck
   end.
 
@@ -696,146 +712,147 @@ Definition check_top_frame (m: mem) (stk: block) (sz: Z) (oldsp: val) ofs_link o
   | _ => false
   end.
 
-Definition exec_instr {exec_load exec_store} `{!MemAccessors exec_load exec_store} {F V} (ge: Genv.t F V) (f: function) (i: instruction) (rs: regset) (m: mem) : outcome :=
-  match i with
+Definition exec_instr {exec_load exec_store} `{!MemAccessors exec_load exec_store} {F V} (ge: Genv.t F V) (f: function) (i: instr_with_info) (rs: regset) (m: mem): outcome :=
+  let sz := snd i in
+  match (fst i) with
   (** Moves *)
   | Pmov_rr rd r1 =>
-      Next (nextinstr (rs#rd <- (rs r1))) m
+      Next (nextinstr (rs#rd <- (rs r1)) sz) m
   | Pmovl_ri rd n =>
-      Next (nextinstr_nf (rs#rd <- (Vint n))) m
+      Next (nextinstr_nf (rs#rd <- (Vint n)) sz) m
   | Pmovq_ri rd n =>
-      Next (nextinstr_nf (rs#rd <- (Vlong n))) m
+      Next (nextinstr_nf (rs#rd <- (Vlong n)) sz) m
   | Pmov_rs rd id =>
-      Next (nextinstr_nf (rs#rd <- (Genv.symbol_address ge id Ptrofs.zero))) m
+      Next (nextinstr_nf (rs#rd <- (Genv.symbol_address ge id Ptrofs.zero)) sz) m
   | Pmovl_rm rd a =>
-      exec_load _ _ ge Mint32 m a rs rd
+      exec_load _ _ ge Mint32 m a rs rd sz
   | Pmovq_rm rd a =>
-      exec_load _ _ ge Mint64 m a rs rd
+      exec_load _ _ ge Mint64 m a rs rd sz
   | Pmovl_mr a r1 =>
-      exec_store _ _ ge Mint32 m a rs r1 nil
+      exec_store _ _ ge Mint32 m a rs r1 nil sz
   | Pmovq_mr a r1 =>
-      exec_store _ _ ge Mint64 m a rs r1 nil
+      exec_store _ _ ge Mint64 m a rs r1 nil sz
   | Pmovsd_ff rd r1 =>
-      Next (nextinstr (rs#rd <- (rs r1))) m
+      Next (nextinstr (rs#rd <- (rs r1)) sz) m
   | Pmovsd_fi rd n =>
-      Next (nextinstr (rs#rd <- (Vfloat n))) m
+      Next (nextinstr (rs#rd <- (Vfloat n)) sz) m
   | Pmovsd_fm rd a =>
-      exec_load _ _ ge Mfloat64 m a rs rd
+      exec_load _ _ ge Mfloat64 m a rs rd sz
   | Pmovsd_mf a r1 =>
-      exec_store _ _ ge Mfloat64 m a rs r1 nil
+      exec_store _ _ ge Mfloat64 m a rs r1 nil sz
   | Pmovss_fi rd n =>
-      Next (nextinstr (rs#rd <- (Vsingle n))) m
+      Next (nextinstr (rs#rd <- (Vsingle n)) sz) m
   | Pmovss_fm rd a =>
-      exec_load _ _ ge Mfloat32 m a rs rd
+      exec_load _ _ ge Mfloat32 m a rs rd sz
   | Pmovss_mf a r1 =>
-      exec_store _ _ ge Mfloat32 m a rs r1 nil
+      exec_store _ _ ge Mfloat32 m a rs r1 nil sz
   | Pfldl_m a =>
-      exec_load _ _ ge Mfloat64 m a rs ST0
+      exec_load _ _ ge Mfloat64 m a rs ST0 sz
   | Pfstpl_m a =>
-      exec_store _ _ ge Mfloat64 m a rs ST0 (ST0 :: nil)
+      exec_store _ _ ge Mfloat64 m a rs ST0 (ST0 :: nil) sz
   | Pflds_m a =>
-      exec_load _ _ ge Mfloat32 m a rs ST0
+      exec_load _ _ ge Mfloat32 m a rs ST0 sz
   | Pfstps_m a =>
-      exec_store _ _ ge Mfloat32 m a rs ST0 (ST0 :: nil)
+      exec_store _ _ ge Mfloat32 m a rs ST0 (ST0 :: nil) sz
   | Pxchg_rr r1 r2 =>
-      Next (nextinstr (rs#r1 <- (rs r2) #r2 <- (rs r1))) m
+      Next (nextinstr (rs#r1 <- (rs r2) #r2 <- (rs r1)) sz) m
   (** Moves with conversion *)
   | Pmovb_mr a r1 =>
-      exec_store _ _ ge Mint8unsigned m a rs r1 nil
+      exec_store _ _ ge Mint8unsigned m a rs r1 nil sz
   | Pmovw_mr a r1 =>
-      exec_store _ _ ge Mint16unsigned m a rs r1 nil
+      exec_store _ _ ge Mint16unsigned m a rs r1 nil sz
   | Pmovzb_rr rd r1 =>
-      Next (nextinstr (rs#rd <- (Val.zero_ext 8 rs#r1))) m
+      Next (nextinstr (rs#rd <- (Val.zero_ext 8 rs#r1)) sz) m 
   | Pmovzb_rm rd a =>
-      exec_load _ _ ge Mint8unsigned m a rs rd
+      exec_load _ _ ge Mint8unsigned m a rs rd sz
   | Pmovsb_rr rd r1 =>
-      Next (nextinstr (rs#rd <- (Val.sign_ext 8 rs#r1))) m
+      Next (nextinstr (rs#rd <- (Val.sign_ext 8 rs#r1)) sz) m
   | Pmovsb_rm rd a =>
-      exec_load _ _ ge Mint8signed m a rs rd
+      exec_load _ _ ge Mint8signed m a rs rd sz
   | Pmovzw_rr rd r1 =>
-      Next (nextinstr (rs#rd <- (Val.zero_ext 16 rs#r1))) m
+      Next (nextinstr (rs#rd <- (Val.zero_ext 16 rs#r1)) sz) m
   | Pmovzw_rm rd a =>
-      exec_load _ _ ge Mint16unsigned m a rs rd
+      exec_load _ _ ge Mint16unsigned m a rs rd sz
   | Pmovsw_rr rd r1 =>
-      Next (nextinstr (rs#rd <- (Val.sign_ext 16 rs#r1))) m
+      Next (nextinstr (rs#rd <- (Val.sign_ext 16 rs#r1)) sz) m
   | Pmovsw_rm rd a =>
-      exec_load _ _ ge Mint16signed m a rs rd
+      exec_load _ _ ge Mint16signed m a rs rd sz
   | Pmovzl_rr rd r1 =>
-      Next (nextinstr (rs#rd <- (Val.longofintu rs#r1))) m
+      Next (nextinstr (rs#rd <- (Val.longofintu rs#r1)) sz) m
   | Pmovsl_rr rd r1 =>
-      Next (nextinstr (rs#rd <- (Val.longofint rs#r1))) m
+      Next (nextinstr (rs#rd <- (Val.longofint rs#r1)) sz) m
   | Pmovls_rr rd =>
-      Next (nextinstr (rs#rd <- (Val.loword rs#rd))) m
+      Next (nextinstr (rs#rd <- (Val.loword rs#rd)) sz) m
   | Pcvtsd2ss_ff rd r1 =>
-      Next (nextinstr (rs#rd <- (Val.singleoffloat rs#r1))) m
+      Next (nextinstr (rs#rd <- (Val.singleoffloat rs#r1)) sz) m
   | Pcvtss2sd_ff rd r1 =>
-      Next (nextinstr (rs#rd <- (Val.floatofsingle rs#r1))) m
+      Next (nextinstr (rs#rd <- (Val.floatofsingle rs#r1)) sz) m
   | Pcvttsd2si_rf rd r1 =>
-      Next (nextinstr (rs#rd <- (Val.maketotal (Val.intoffloat rs#r1)))) m
+      Next (nextinstr (rs#rd <- (Val.maketotal (Val.intoffloat rs#r1))) sz) m
   | Pcvtsi2sd_fr rd r1 =>
-      Next (nextinstr (rs#rd <- (Val.maketotal (Val.floatofint rs#r1)))) m
+      Next (nextinstr (rs#rd <- (Val.maketotal (Val.floatofint rs#r1))) sz) m
   | Pcvttss2si_rf rd r1 =>
-      Next (nextinstr (rs#rd <- (Val.maketotal (Val.intofsingle rs#r1)))) m
+      Next (nextinstr (rs#rd <- (Val.maketotal (Val.intofsingle rs#r1))) sz) m
   | Pcvtsi2ss_fr rd r1 =>
-      Next (nextinstr (rs#rd <- (Val.maketotal (Val.singleofint rs#r1)))) m
+      Next (nextinstr (rs#rd <- (Val.maketotal (Val.singleofint rs#r1))) sz) m
   | Pcvttsd2sl_rf rd r1 =>
-      Next (nextinstr (rs#rd <- (Val.maketotal (Val.longoffloat rs#r1)))) m
+      Next (nextinstr (rs#rd <- (Val.maketotal (Val.longoffloat rs#r1))) sz) m
   | Pcvtsl2sd_fr rd r1 =>
-      Next (nextinstr (rs#rd <- (Val.maketotal (Val.floatoflong rs#r1)))) m
+      Next (nextinstr (rs#rd <- (Val.maketotal (Val.floatoflong rs#r1))) sz) m
   | Pcvttss2sl_rf rd r1 =>
-      Next (nextinstr (rs#rd <- (Val.maketotal (Val.longofsingle rs#r1)))) m
+      Next (nextinstr (rs#rd <- (Val.maketotal (Val.longofsingle rs#r1))) sz) m
   | Pcvtsl2ss_fr rd r1 =>
-      Next (nextinstr (rs#rd <- (Val.maketotal (Val.singleoflong rs#r1)))) m
+      Next (nextinstr (rs#rd <- (Val.maketotal (Val.singleoflong rs#r1))) sz) m
   (** Integer arithmetic *)
   | Pleal rd a =>
-      Next (nextinstr (rs#rd <- (eval_addrmode32 ge a rs))) m
+      Next (nextinstr (rs#rd <- (eval_addrmode32 ge a rs)) sz) m
   | Pleaq rd a =>
-      Next (nextinstr (rs#rd <- (eval_addrmode64 ge a rs))) m
+      Next (nextinstr (rs#rd <- (eval_addrmode64 ge a rs)) sz) m
   | Pnegl rd =>
-      Next (nextinstr_nf (rs#rd <- (Val.neg rs#rd))) m
+      Next (nextinstr_nf (rs#rd <- (Val.neg rs#rd)) sz) m
   | Pnegq rd =>
-      Next (nextinstr_nf (rs#rd <- (Val.negl rs#rd))) m
+      Next (nextinstr_nf (rs#rd <- (Val.negl rs#rd)) sz) m
   | Paddl_ri rd n =>
-      Next (nextinstr_nf (rs#rd <- (Val.add rs#rd (Vint n)))) m
+      Next (nextinstr_nf (rs#rd <- (Val.add rs#rd (Vint n)))sz ) m
   | Psubl_ri rd n =>
-    Next (nextinstr_nf (rs#rd <- (Val.sub rs#rd (Vint n)))) m
+    Next (nextinstr_nf (rs#rd <- (Val.sub rs#rd (Vint n))) sz) m
   | Paddq_ri rd n =>
-    Next (nextinstr_nf (rs#rd <- (Val.addl rs#rd (Vlong n)))) m
+    Next (nextinstr_nf (rs#rd <- (Val.addl rs#rd (Vlong n))) sz) m
   | Psubq_ri rd n =>
-    Next (nextinstr_nf (rs#rd <- (Val.subl rs#rd (Vlong n)))) m
+    Next (nextinstr_nf (rs#rd <- (Val.subl rs#rd (Vlong n)))sz ) m
   | Psubl_rr rd r1 =>
-      Next (nextinstr_nf (rs#rd <- (Val.sub rs#rd rs#r1))) m
+      Next (nextinstr_nf (rs#rd <- (Val.sub rs#rd rs#r1)) sz) m
   | Psubq_rr rd r1 =>
-      Next (nextinstr_nf (rs#rd <- (Val.subl rs#rd rs#r1))) m
+      Next (nextinstr_nf (rs#rd <- (Val.subl rs#rd rs#r1)) sz) m
   | Pimull_rr rd r1 =>
-      Next (nextinstr_nf (rs#rd <- (Val.mul rs#rd rs#r1))) m
+      Next (nextinstr_nf (rs#rd <- (Val.mul rs#rd rs#r1)) sz) m
   | Pimulq_rr rd r1 =>
-      Next (nextinstr_nf (rs#rd <- (Val.mull rs#rd rs#r1))) m
+      Next (nextinstr_nf (rs#rd <- (Val.mull rs#rd rs#r1)) sz) m
   | Pimull_ri rd n =>
-      Next (nextinstr_nf (rs#rd <- (Val.mul rs#rd (Vint n)))) m
+      Next (nextinstr_nf (rs#rd <- (Val.mul rs#rd (Vint n))) sz) m
   | Pimulq_ri rd n =>
-      Next (nextinstr_nf (rs#rd <- (Val.mull rs#rd (Vlong n)))) m
+      Next (nextinstr_nf (rs#rd <- (Val.mull rs#rd (Vlong n))) sz) m
   | Pimull_r r1 =>
       Next (nextinstr_nf (rs#RAX <- (Val.mul rs#RAX rs#r1)
-                            #RDX <- (Val.mulhs rs#RAX rs#r1))) m
+                            #RDX <- (Val.mulhs rs#RAX rs#r1)) sz) m
   | Pimulq_r r1 =>
       Next (nextinstr_nf (rs#RAX <- (Val.mull rs#RAX rs#r1)
-                            #RDX <- (Val.mullhs rs#RAX rs#r1))) m
+                            #RDX <- (Val.mullhs rs#RAX rs#r1)) sz) m
   | Pmull_r r1 =>
       Next (nextinstr_nf (rs#RAX <- (Val.mul rs#RAX rs#r1)
-                            #RDX <- (Val.mulhu rs#RAX rs#r1))) m
+                            #RDX <- (Val.mulhu rs#RAX rs#r1)) sz) m
   | Pmulq_r r1 =>
       Next (nextinstr_nf (rs#RAX <- (Val.mull rs#RAX rs#r1)
-                            #RDX <- (Val.mullhu rs#RAX rs#r1))) m
+                            #RDX <- (Val.mullhu rs#RAX rs#r1)) sz) m
   | Pcltd =>
-      Next (nextinstr_nf (rs#RDX <- (Val.shr rs#RAX (Vint (Int.repr 31))))) m
+      Next (nextinstr_nf (rs#RDX <- (Val.shr rs#RAX (Vint (Int.repr 31)))) sz) m
   | Pcqto =>
-      Next (nextinstr_nf (rs#RDX <- (Val.shrl rs#RAX (Vint (Int.repr 63))))) m
+      Next (nextinstr_nf (rs#RDX <- (Val.shrl rs#RAX (Vint (Int.repr 63)))) sz) m
   | Pdivl r1 =>
       match rs#RDX, rs#RAX, rs#r1 with
       | Vint nh, Vint nl, Vint d =>
           match Int.divmodu2 nh nl d with
-          | Some(q, r) => Next (nextinstr_nf (rs#RAX <- (Vint q) #RDX <- (Vint r))) m
+          | Some(q, r) => Next (nextinstr_nf (rs#RAX <- (Vint q) #RDX <- (Vint r)) sz) m
           | None => Stuck
           end
       | _, _, _ => Stuck
@@ -844,7 +861,7 @@ Definition exec_instr {exec_load exec_store} `{!MemAccessors exec_load exec_stor
       match rs#RDX, rs#RAX, rs#r1 with
       | Vlong nh, Vlong nl, Vlong d =>
           match Int64.divmodu2 nh nl d with
-          | Some(q, r) => Next (nextinstr_nf (rs#RAX <- (Vlong q) #RDX <- (Vlong r))) m
+          | Some(q, r) => Next (nextinstr_nf (rs#RAX <- (Vlong q) #RDX <- (Vlong r)) sz) m
           | None => Stuck
           end
       | _, _, _ => Stuck
@@ -853,7 +870,7 @@ Definition exec_instr {exec_load exec_store} `{!MemAccessors exec_load exec_stor
       match rs#RDX, rs#RAX, rs#r1 with
       | Vint nh, Vint nl, Vint d =>
           match Int.divmods2 nh nl d with
-          | Some(q, r) => Next (nextinstr_nf (rs#RAX <- (Vint q) #RDX <- (Vint r))) m
+          | Some(q, r) => Next (nextinstr_nf (rs#RAX <- (Vint q) #RDX <- (Vint r)) sz) m
           | None => Stuck
           end
       | _, _, _ => Stuck
@@ -862,133 +879,133 @@ Definition exec_instr {exec_load exec_store} `{!MemAccessors exec_load exec_stor
       match rs#RDX, rs#RAX, rs#r1 with
       | Vlong nh, Vlong nl, Vlong d =>
           match Int64.divmods2 nh nl d with
-          | Some(q, r) => Next (nextinstr_nf (rs#RAX <- (Vlong q) #RDX <- (Vlong r))) m
+          | Some(q, r) => Next (nextinstr_nf (rs#RAX <- (Vlong q) #RDX <- (Vlong r)) sz) m
           | None => Stuck
           end
       | _, _, _ => Stuck
       end
   | Pandl_rr rd r1 =>
-      Next (nextinstr_nf (rs#rd <- (Val.and rs#rd rs#r1))) m
+      Next (nextinstr_nf (rs#rd <- (Val.and rs#rd rs#r1)) sz) m
   | Pandq_rr rd r1 =>
-      Next (nextinstr_nf (rs#rd <- (Val.andl rs#rd rs#r1))) m
+      Next (nextinstr_nf (rs#rd <- (Val.andl rs#rd rs#r1)) sz) m
   | Pandl_ri rd n =>
-      Next (nextinstr_nf (rs#rd <- (Val.and rs#rd (Vint n)))) m
+      Next (nextinstr_nf (rs#rd <- (Val.and rs#rd (Vint n))) sz) m
   | Pandq_ri rd n =>
-      Next (nextinstr_nf (rs#rd <- (Val.andl rs#rd (Vlong n)))) m
+      Next (nextinstr_nf (rs#rd <- (Val.andl rs#rd (Vlong n))) sz) m
   | Porl_rr rd r1 =>
-      Next (nextinstr_nf (rs#rd <- (Val.or rs#rd rs#r1))) m
+      Next (nextinstr_nf (rs#rd <- (Val.or rs#rd rs#r1)) sz) m
   | Porq_rr rd r1 =>
-      Next (nextinstr_nf (rs#rd <- (Val.orl rs#rd rs#r1))) m
+      Next (nextinstr_nf (rs#rd <- (Val.orl rs#rd rs#r1)) sz) m
   | Porl_ri rd n =>
-      Next (nextinstr_nf (rs#rd <- (Val.or rs#rd (Vint n)))) m
+      Next (nextinstr_nf (rs#rd <- (Val.or rs#rd (Vint n))) sz) m
   | Porq_ri rd n =>
-      Next (nextinstr_nf (rs#rd <- (Val.orl rs#rd (Vlong n)))) m
+      Next (nextinstr_nf (rs#rd <- (Val.orl rs#rd (Vlong n))) sz) m
   | Pxorl_r rd =>
-      Next (nextinstr_nf (rs#rd <- Vzero)) m
+      Next (nextinstr_nf (rs#rd <- Vzero) sz) m
   | Pxorq_r rd =>
-      Next (nextinstr_nf (rs#rd <- (Vlong Int64.zero))) m
+      Next (nextinstr_nf (rs#rd <- (Vlong Int64.zero)) sz) m
   | Pxorl_rr rd r1 =>
-      Next (nextinstr_nf (rs#rd <- (Val.xor rs#rd rs#r1))) m
+      Next (nextinstr_nf (rs#rd <- (Val.xor rs#rd rs#r1))sz) m
   | Pxorq_rr rd r1 =>
-      Next (nextinstr_nf (rs#rd <- (Val.xorl rs#rd rs#r1))) m 
+      Next (nextinstr_nf (rs#rd <- (Val.xorl rs#rd rs#r1)) sz) m 
   | Pxorl_ri rd n =>
-      Next (nextinstr_nf (rs#rd <- (Val.xor rs#rd (Vint n)))) m
+      Next (nextinstr_nf (rs#rd <- (Val.xor rs#rd (Vint n))) sz) m
   | Pxorq_ri rd n =>
-      Next (nextinstr_nf (rs#rd <- (Val.xorl rs#rd (Vlong n)))) m
+      Next (nextinstr_nf (rs#rd <- (Val.xorl rs#rd (Vlong n))) sz) m
   | Pnotl rd =>
-      Next (nextinstr_nf (rs#rd <- (Val.notint rs#rd))) m
+      Next (nextinstr_nf (rs#rd <- (Val.notint rs#rd)) sz) m
   | Pnotq rd =>
-      Next (nextinstr_nf (rs#rd <- (Val.notl rs#rd))) m
+      Next (nextinstr_nf (rs#rd <- (Val.notl rs#rd)) sz) m
   | Psall_rcl rd =>
-      Next (nextinstr_nf (rs#rd <- (Val.shl rs#rd rs#RCX))) m
+      Next (nextinstr_nf (rs#rd <- (Val.shl rs#rd rs#RCX)) sz) m
   | Psalq_rcl rd =>
-      Next (nextinstr_nf (rs#rd <- (Val.shll rs#rd rs#RCX))) m
+      Next (nextinstr_nf (rs#rd <- (Val.shll rs#rd rs#RCX)) sz) m
   | Psall_ri rd n =>
-      Next (nextinstr_nf (rs#rd <- (Val.shl rs#rd (Vint n)))) m
+      Next (nextinstr_nf (rs#rd <- (Val.shl rs#rd (Vint n))) sz) m
   | Psalq_ri rd n =>
-      Next (nextinstr_nf (rs#rd <- (Val.shll rs#rd (Vint n)))) m
+      Next (nextinstr_nf (rs#rd <- (Val.shll rs#rd (Vint n))) sz) m
   | Pshrl_rcl rd =>
-      Next (nextinstr_nf (rs#rd <- (Val.shru rs#rd rs#RCX))) m
+      Next (nextinstr_nf (rs#rd <- (Val.shru rs#rd rs#RCX)) sz) m
   | Pshrq_rcl rd =>
-      Next (nextinstr_nf (rs#rd <- (Val.shrlu rs#rd rs#RCX))) m
+      Next (nextinstr_nf (rs#rd <- (Val.shrlu rs#rd rs#RCX)) sz) m
   | Pshrl_ri rd n =>
-      Next (nextinstr_nf (rs#rd <- (Val.shru rs#rd (Vint n)))) m
+      Next (nextinstr_nf (rs#rd <- (Val.shru rs#rd (Vint n))) sz) m
   | Pshrq_ri rd n =>
-      Next (nextinstr_nf (rs#rd <- (Val.shrlu rs#rd (Vint n)))) m
+      Next (nextinstr_nf (rs#rd <- (Val.shrlu rs#rd (Vint n))) sz) m
   | Psarl_rcl rd =>
-      Next (nextinstr_nf (rs#rd <- (Val.shr rs#rd rs#RCX))) m
+      Next (nextinstr_nf (rs#rd <- (Val.shr rs#rd rs#RCX)) sz) m
   | Psarq_rcl rd =>
-      Next (nextinstr_nf (rs#rd <- (Val.shrl rs#rd rs#RCX))) m
+      Next (nextinstr_nf (rs#rd <- (Val.shrl rs#rd rs#RCX)) sz) m
   | Psarl_ri rd n =>
-      Next (nextinstr_nf (rs#rd <- (Val.shr rs#rd (Vint n)))) m
+      Next (nextinstr_nf (rs#rd <- (Val.shr rs#rd (Vint n))) sz) m
   | Psarq_ri rd n =>
-      Next (nextinstr_nf (rs#rd <- (Val.shrl rs#rd (Vint n)))) m
+      Next (nextinstr_nf (rs#rd <- (Val.shrl rs#rd (Vint n))) sz) m
   | Pshld_ri rd r1 n =>
       Next (nextinstr_nf
               (rs#rd <- (Val.or (Val.shl rs#rd (Vint n))
-                                (Val.shru rs#r1 (Vint (Int.sub Int.iwordsize n)))))) m
+                                (Val.shru rs#r1 (Vint (Int.sub Int.iwordsize n))))) sz) m
   | Prorl_ri rd n =>
-      Next (nextinstr_nf (rs#rd <- (Val.ror rs#rd (Vint n)))) m
+      Next (nextinstr_nf (rs#rd <- (Val.ror rs#rd (Vint n))) sz) m
   | Prorq_ri rd n =>
-      Next (nextinstr_nf (rs#rd <- (Val.rorl rs#rd (Vint n)))) m
+      Next (nextinstr_nf (rs#rd <- (Val.rorl rs#rd (Vint n))) sz) m
   | Pcmpl_rr r1 r2 =>
-      Next (nextinstr (compare_ints (rs r1) (rs r2) rs m)) m
+      Next (nextinstr (compare_ints (rs r1) (rs r2) rs m) sz) m
   | Pcmpq_rr r1 r2 =>
-      Next (nextinstr (compare_longs (rs r1) (rs r2) rs m)) m
+      Next (nextinstr (compare_longs (rs r1) (rs r2) rs m) sz) m
   | Pcmpl_ri r1 n =>
-      Next (nextinstr (compare_ints (rs r1) (Vint n) rs m)) m
+      Next (nextinstr (compare_ints (rs r1) (Vint n) rs m) sz) m
   | Pcmpq_ri r1 n =>
-      Next (nextinstr (compare_longs (rs r1) (Vlong n) rs m)) m
+      Next (nextinstr (compare_longs (rs r1) (Vlong n) rs m) sz) m
   | Ptestl_rr r1 r2 =>
-      Next (nextinstr (compare_ints (Val.and (rs r1) (rs r2)) Vzero rs m)) m
+      Next (nextinstr (compare_ints (Val.and (rs r1) (rs r2)) Vzero rs m) sz) m
   | Ptestq_rr r1 r2 =>
-      Next (nextinstr (compare_longs (Val.andl (rs r1) (rs r2)) (Vlong Int64.zero) rs m)) m
+      Next (nextinstr (compare_longs (Val.andl (rs r1) (rs r2)) (Vlong Int64.zero) rs m) sz) m
   | Ptestl_ri r1 n =>
-      Next (nextinstr (compare_ints (Val.and (rs r1) (Vint n)) Vzero rs m)) m
+      Next (nextinstr (compare_ints (Val.and (rs r1) (Vint n)) Vzero rs m) sz) m
   | Ptestq_ri r1 n =>
-      Next (nextinstr (compare_longs (Val.andl (rs r1) (Vlong n)) (Vlong Int64.zero) rs m)) m
+      Next (nextinstr (compare_longs (Val.andl (rs r1) (Vlong n)) (Vlong Int64.zero) rs m) sz) m
   | Pcmov c rd r1 =>
       match eval_testcond c rs with
-      | Some true => Next (nextinstr (rs#rd <- (rs#r1))) m
-      | Some false => Next (nextinstr rs) m
-      | None => Next (nextinstr (rs#rd <- Vundef)) m
+      | Some true => Next (nextinstr (rs#rd <- (rs#r1)) sz) m
+      | Some false => Next (nextinstr rs sz) m
+      | None => Next (nextinstr (rs#rd <- Vundef) sz) m
       end
   | Psetcc c rd =>
-      Next (nextinstr (rs#rd <- (Val.of_optbool (eval_testcond c rs)))) m
+      Next (nextinstr (rs#rd <- (Val.of_optbool (eval_testcond c rs))) sz) m
   (** Arithmetic operations over double-precision floats *)
   | Paddd_ff rd r1 =>
-      Next (nextinstr (rs#rd <- (Val.addf rs#rd rs#r1))) m
+      Next (nextinstr (rs#rd <- (Val.addf rs#rd rs#r1)) sz) m
   | Psubd_ff rd r1 =>
-      Next (nextinstr (rs#rd <- (Val.subf rs#rd rs#r1))) m
+      Next (nextinstr (rs#rd <- (Val.subf rs#rd rs#r1)) sz) m
   | Pmuld_ff rd r1 =>
-      Next (nextinstr (rs#rd <- (Val.mulf rs#rd rs#r1))) m
+      Next (nextinstr (rs#rd <- (Val.mulf rs#rd rs#r1)) sz) m
   | Pdivd_ff rd r1 =>
-      Next (nextinstr (rs#rd <- (Val.divf rs#rd rs#r1))) m
+      Next (nextinstr (rs#rd <- (Val.divf rs#rd rs#r1)) sz) m
   | Pnegd rd =>
-      Next (nextinstr (rs#rd <- (Val.negf rs#rd))) m
+      Next (nextinstr (rs#rd <- (Val.negf rs#rd)) sz) m
   | Pabsd rd =>
-      Next (nextinstr (rs#rd <- (Val.absf rs#rd))) m
+      Next (nextinstr (rs#rd <- (Val.absf rs#rd)) sz) m
   | Pcomisd_ff r1 r2 =>
-      Next (nextinstr (compare_floats (rs r1) (rs r2) rs)) m
+      Next (nextinstr (compare_floats (rs r1) (rs r2) rs) sz) m
   | Pxorpd_f rd =>
-      Next (nextinstr_nf (rs#rd <- (Vfloat Float.zero))) m
+      Next (nextinstr_nf (rs#rd <- (Vfloat Float.zero)) sz) m
   (** Arithmetic operations over single-precision floats *)
   | Padds_ff rd r1 =>
-      Next (nextinstr (rs#rd <- (Val.addfs rs#rd rs#r1))) m
+      Next (nextinstr (rs#rd <- (Val.addfs rs#rd rs#r1)) sz) m
   | Psubs_ff rd r1 =>
-      Next (nextinstr (rs#rd <- (Val.subfs rs#rd rs#r1))) m
+      Next (nextinstr (rs#rd <- (Val.subfs rs#rd rs#r1)) sz) m
   | Pmuls_ff rd r1 =>
-      Next (nextinstr (rs#rd <- (Val.mulfs rs#rd rs#r1))) m
+      Next (nextinstr (rs#rd <- (Val.mulfs rs#rd rs#r1)) sz) m
   | Pdivs_ff rd r1 =>
-      Next (nextinstr (rs#rd <- (Val.divfs rs#rd rs#r1))) m
+      Next (nextinstr (rs#rd <- (Val.divfs rs#rd rs#r1)) sz) m
   | Pnegs rd =>
-      Next (nextinstr (rs#rd <- (Val.negfs rs#rd))) m
+      Next (nextinstr (rs#rd <- (Val.negfs rs#rd)) sz) m
   | Pabss rd =>
-      Next (nextinstr (rs#rd <- (Val.absfs rs#rd))) m
+      Next (nextinstr (rs#rd <- (Val.absfs rs#rd)) sz) m
   | Pcomiss_ff r1 r2 =>
-      Next (nextinstr (compare_floats32 (rs r1) (rs r2) rs)) m
+      Next (nextinstr (compare_floats32 (rs r1) (rs r2) rs) sz) m
   | Pxorps_f rd =>
-      Next (nextinstr_nf (rs#rd <- (Vsingle Float32.zero))) m
+      Next (nextinstr_nf (rs#rd <- (Vsingle Float32.zero)) sz) m
   (** Branches and calls *)
   | Pjmp_l lbl =>
       goto_label ge f lbl rs m
@@ -999,13 +1016,13 @@ Definition exec_instr {exec_load exec_store} `{!MemAccessors exec_load exec_stor
   | Pjcc cond lbl =>
       match eval_testcond cond rs with
       | Some true => goto_label ge f lbl rs m
-      | Some false => Next (nextinstr rs) m
+      | Some false => Next (nextinstr rs sz) m
       | None => Stuck
       end
   | Pjcc2 cond1 cond2 lbl =>
       match eval_testcond cond1 rs, eval_testcond cond2 rs with
       | Some true, Some true => goto_label ge f lbl rs m
-      | Some _, Some _ => Next (nextinstr rs) m
+      | Some _, Some _ => Next (nextinstr rs sz) m
       | _, _ => Stuck
       end
   | Pjmptbl r tbl =>
@@ -1027,25 +1044,25 @@ Definition exec_instr {exec_load exec_store} `{!MemAccessors exec_load exec_stor
       Next (rs#PC <- (rs#RA) #RA <- Vundef) m
   (** Saving and restoring registers *)
   | Pmov_rm_a rd a =>
-      exec_load _ _ ge (if Archi.ptr64 then Many64 else Many32) m a rs rd
+      exec_load _ _ ge (if Archi.ptr64 then Many64 else Many32) m a rs rd sz
   | Pmov_mr_a a r1 =>
-      exec_store _ _ ge (if Archi.ptr64 then Many64 else Many32) m a rs r1 nil
+      exec_store _ _ ge (if Archi.ptr64 then Many64 else Many32) m a rs r1 nil sz
   | Pmovsd_fm_a rd a =>
-      exec_load _ _ ge Many64 m a rs rd
+      exec_load _ _ ge Many64 m a rs rd sz
   | Pmovsd_mf_a a r1 =>
-      exec_store _ _ ge Many64 m a rs r1 nil
+      exec_store _ _ ge Many64 m a rs r1 nil sz
   (** Pseudo-instructions *)
   | Plabel lbl =>
-      Next (nextinstr rs) m
+      Next (nextinstr rs sz) m
   | Pallocframe fi ofs_ra ofs_link =>
     if check_alloc_frame fi ofs_link ofs_ra then
       match Mem.push_frame m fi ((Mptr, ofs_link, rs#RSP)::(Mptr,ofs_ra, rs#RA)::nil) with
         Some (m4,b) =>
-        Next (nextinstr (rs #RAX <- (rs#RSP) #RSP <- (Vptr b Ptrofs.zero))) m4
+        Next (nextinstr (rs #RAX <- (rs#RSP) #RSP <- (Vptr b Ptrofs.zero)) sz) m4
       | _ => Stuck
       end
     else Stuck
-  | Pfreeframe sz ofs_ra ofs_link =>
+  | Pfreeframe sz' ofs_ra ofs_link =>
       match Mem.loadv Mptr m (Val.offset_ptr rs#RSP ofs_ra) with
       | None => Stuck
       | Some ra =>
@@ -1054,13 +1071,13 @@ Definition exec_instr {exec_load exec_store} `{!MemAccessors exec_load exec_stor
           | Some sp =>
               match rs#RSP with
               | Vptr stk ofs =>
-                if check_top_frame m stk sz sp ofs_link ofs_ra
+                if check_top_frame m stk sz' sp ofs_link ofs_ra
                 then
-                  match Mem.free m stk 0 sz with
+                  match Mem.free m stk 0 sz' with
                   | None => Stuck
                   | Some m' =>
                     match Mem.unrecord_stack_block m' with
-                      Some m' => Next (nextinstr (rs#RSP <- sp #RA <- ra)) m'
+                      Some m' => Next (nextinstr (rs#RSP <- sp #RA <- ra) sz) m'
                     | None => Stuck
                     end
                   end
@@ -1111,8 +1128,6 @@ Definition exec_instr {exec_load exec_store} `{!MemAccessors exec_load exec_stor
   | Psqrtsd _ _
     => Stuck
   end.
-
-End WITH_FIND_LABELS.
 
 
 
@@ -1189,7 +1204,8 @@ Definition loc_external_result (sg: signature) : rpair preg :=
 Inductive state {memory_model_ops: Mem.MemoryModelOps mem}: Type :=
   | State: regset -> mem -> state.
 
-Inductive step {exec_load exec_store} `{!MemAccessors exec_load exec_store} (ge: genv) : state -> trace -> state -> Prop :=
+Inductive step {exec_load exec_store} `{!MemAccessors exec_load exec_store} (ge: genv)
+            : state -> trace -> state -> Prop :=
 | exec_step_internal:
     forall b ofs f i rs m rs' m',
       rs PC = Vptr b ofs ->
@@ -1198,17 +1214,18 @@ Inductive step {exec_load exec_store} `{!MemAccessors exec_load exec_store} (ge:
       exec_instr ge f i rs m = Next rs' m' ->
       step ge (State rs m) E0 (State rs' m')
 | exec_step_builtin:
-    forall b ofs f ef args res rs m vargs t vres rs' m',
+    forall b ofs f ef args res rs m vargs t vres rs' m' sz,
       rs PC = Vptr b ofs ->
       Genv.find_funct_ptr ge b = Some (Internal f) ->
-      find_instr (Ptrofs.unsigned ofs) f.(fn_code) = Some (Pbuiltin ef args res) ->
+      find_instr (Ptrofs.unsigned ofs) f.(fn_code) = Some (Pbuiltin ef args res, sz) ->
       eval_builtin_args ge rs (rs RSP) m args vargs ->
       external_call ef ge vargs m t vres m' ->
       forall BUILTIN_ENABLED: builtin_enabled ef,
         no_rsp_builtin_preg res ->
         rs' = nextinstr_nf
                 (set_res res vres
-                         (undef_regs (map preg_of (destroyed_by_builtin ef)) rs)) ->
+                         (undef_regs (map preg_of (destroyed_by_builtin ef)) rs))
+                sz ->
         step ge (State rs m) t (State rs' m')
 | exec_step_external:
     forall b ef args res rs m t rs' m',
